proof/equivFake.ec
@@ -12,23 +12,96 @@ require import Gate.
 require import GarbleTools.
 require AdvGate.
 
-require import Bitstring.
-require import Int.
-require import Bool.
-require import Pair.
-require import Map.
-require import Distr.
-require import List.
+module Fake(Adv:Gate.Adv) = {
+  fun fake() : bool = {
+    var c : bool;
+    var query : Gate.query;
+    var ret : Dkc.query list;
+    var challenge : bool;
+    var gg : Gate.functG;
+    var query0 : Gate.funct*Gate.input;
+    var query1 : Gate.funct*Gate.input;
+    var v : bool;
 
-require import Dkc.
-require import Gate.
-require import GarbleTools.
+    var rand : bool;
+    var ntau : bool;
+    var t : bool;
+    var keyt : token;
+    var keynt : token;
+    var keytau : token;
+    var keyntau : token;
+    var key_t_tau : token;
+    var key_nt_ntau : token;
+    var key_nt_tau : token;
+    var key_t_ntau : token;
+
+    var input : Gate.inputG;
+    var g : ((bool*bool), token) map;
+
+    (* t^^(fst xc) = t *)
+    (* !tau = ntau *)
+
+    ntau = $Dbool.dbool;
+    keytau = $Dkc.genRandKeyLast(!ntau);
+
+    query := AdvGate.A.gen_query();
+    query0 = fst query;
+    query1 = snd query;
+    if (Gate.eval (fst query0) (snd query0) = Gate.eval (fst query0) (snd query0))
+    {
+    v = Gate.eval (fst query0) (snd query0);
+    
+    t = $Dbool.dbool;
+
+    keyt = $Dkc.genRandKeyLast(t);
+    key_t_tau = $Dkc.genRandKey;
+
+    keynt = $Dkc.genRandKeyLast(!t);
+    key_nt_tau = $Dkc.genRandKey;
+
+    key_t_ntau = $Dkc.genRandKeyLast(v);
+
+    keyntau = $Dkc.genRandKeyLast(ntau);
+    key_nt_ntau  = $Dkc.genRandKey;
+
+    input = (keyt, keyntau);
+    
+    g.[(  ntau,  t)] = Dkc.encode
+      (tweak 2 ( ntau) ( t))
+      keyntau
+      keyt
+      key_t_ntau;
+    g.[(  ntau, !t)] = Dkc.encode
+      (tweak 2 ( ntau) (!t))
+      keyntau
+      keynt
+      key_nt_ntau;
+    g.[( !ntau,  t)] = Dkc.encode
+      (tweak 2 (!ntau) ( t))
+      keytau
+      keyt
+      key_t_tau;
+    g.[( !ntau,  !t)] = Dkc.encode
+      (tweak 2 (!ntau) (!t))
+      keytau
+      keynt
+      key_nt_tau;
+
+    gg = (proj g.[(false, false)], proj g.[(false, true)], proj g.[(true, false)], proj g.[(true, true)]);
+    challenge := AdvGate.A.get_challenge((gg, input, tt));
+    }
+    else
+      challenge = $Dbool.dbool;
+    c = $Dbool.dbool;
+    return c = challenge;
+  }
+}.
 
 lemma FakeEq :
   forall (Adv <: Gate.Adv),
     equiv [
-      Dkc.Game(Dkc.Dkc, AdvGate.Adv(Adv)).work ~ AdvGate.Adv(Adv).fake :
-      (! Dkc.Dkc.b{1}) /\ (AdvGate.Adv.l{1}=1) /\ (Dkc.Dkc.b{2}) /\ (AdvGate.Adv.l{2}=2) ==> res{1} = res{2}
+      Dkc.Game(Dkc.Dkc, AdvGate.Adv(Adv)).work ~ Fake(Adv).fake :
+      (! Dkc.Dkc.b{1}) /\ (AdvGate.Adv.l{1}=1) ==> res{1} = res{2}
     ]
 proof.
   intros Adv.
@@ -38,33 +111,170 @@ proof.
   inline {1} Dkc.Dkc.initialize.
   inline {1} AdvGate.Adv.gen_queries.
   inline {1} AdvGate.Adv.get_challenge.
-  rcondf {1} 9;[admit|].
-  rcondt {1} 9;[admit|].
-  rcondf {1} 17;[admit|].
-  rcondt {1} 17;[admit|].
+  rcondf {1} 11;[admit|]. (* l condition *)
+  rcondt {1} 11;[admit|]. (* l condition *)
+  rcondf {1} 19;[admit|]. (* l condition *)
+  rcondt {1} 19;[admit|]. (* l condition *)
   inline {1} AdvGate.Adv.compute1.
   inline {1} AdvGate.Adv.gen_queries1.
-  rcondt {1} 15;[admit|].
-  rcondf {1} 18;[admit|].
+  rcondt {1} 18;[admit|]. (* While *)
+  rcondt {1} 21;[admit|]. (* While *)
+  rcondf {1} 24;[admit|]. (* While *)
   inline {1} Dkc.Dkc.encrypt.
 
   wp.
-  swap {2} 22 -20.
-  call (answer{1}=answer{2}) (res{1} = res{2}). admit.
+  swap {2} 7 -4.
+  rcondt {2} 7. admit. (*FAUX*) (*BAD Condition*)
+  call (answer{1}=answer{2}) (res{1} = res{2}). admit. (* Call Adv get_challenge *)
   wp.
-  rnd.
-  rnd.
-  rnd.
-  rnd.
+  rnd. (* key_nt_ntau *)
+  rnd. (* keyntau *)
+  wp.
+  rcondf {1} 37. admit. (*FAUX*) (* Reutilisation clef sortie *)
+  rcondf {1} 37. admit. (*FAUX*) (* Reutilisation clef sortie *)
+  rnd. (* key_t_ntau *)
+  wp.
+
+  (*BEGIN DKC*)
+  (*LOOP 1*)
+  rcondt {1} 28. admit. (* Dkc used *)
+  wp.
+  rcondt {1} 29. admit. (* Dkc not reusing *)
+  rcondf {1} 30. admit. (* Dkc not reusing *)
+  rcondt {1} 30. admit. (* Dkc not reusing *)
+  rnd. (* key_nt_tau *)
+  rnd. (* keynt *)
+  wp.
+  (*LOOP 2*)
+  rcondt {1} 21. admit. (* Dkc used *)
+  wp.
+  rcondt {1} 22. admit. (* Dkc not reusing *)
+  rcondf {1} 23. admit. (* Dkc not reusing *)
+  rcondt {1} 23. admit. (* Dkc not reusing *)
+  rnd. (* key_t_tau *)
+  rnd. (* keyt *)
+  wp.
+  (*END DKC*)
+  rnd {1}. (* rand *)
+  rnd (lambda x, x^^(fst AdvGate.Adv.xc{1})) _. (* t *)
+  wp.
+  call true (res{1} = res{2}). admit. (* Call Adv gen_query *)
+  rnd. (* c *)
+  wp.
+  rnd. (*keyTau*)
+  rnd (lambda x, !x) _. (*tau*)
+
+  skip.
+
+  intros &1 &2 pre.
+  simplify.
+  intros tau1 ntau2; split;[trivial|];intros eqtau intau.
+  intros keyTau1 keyTau2;split;[trivial|];intros eqKeyTau inKeyTau.
+  intros c1 c2;split;[trivial|];intros eqc inc.  
+  intros query1 query2 eqQuery.
+  case c1;intros c1val.
+    intros t1 t2; split;[trivial|];intros eqt int.
+    intros rand inrand.
+
+    (* UGLY *)
+    rewrite (hd_def<:(int*bool)*(int*bool)*bool*(bool array)> ((0, t1 ^^ fst (snd (fst query1))),
+    (1,
+      eval (fst (fst query1)) (fst (snd (fst query1)),
+        !snd (snd (fst query1)))),
+      false, tweak 0 (!t1 ^^ (fst (snd (fst query1)))) tau1)
+(
+    (((0, !t1 ^^ fst (snd (fst query1))),
+      (2, rand), false, tweak 0 (!t1 ^^ fst (snd (fst query1))) tau1) ::
+      __nil))).
+    (* END UGLY *)
+
+    simplify.
+    intros keyt1 keyt2; split;[trivial|];intros eqkeyt inkeyt.
+    intros key_t_tau inkey_t_tau.
+
+    (* UGLY *)
+    rewrite (tl_def<:(int*bool)*(int*bool)*bool*(bool array)> ((0, t1 ^^ fst (snd (fst query1))),
+    (1,
+      eval (fst (fst query1)) (fst (snd (fst query1)),
+        !snd (snd (fst query1)))),
+      false, tweak 0 (!t1 ^^ (fst (snd (fst query1)))) tau1)
+(
+    (((0, !t1 ^^ fst (snd (fst query1))),
+      (2, rand), false, tweak 0 (!t1 ^^ fst (snd (fst query1))) tau1) ::
+      __nil))).
+    rewrite (hd_def<:(int*bool)*(int*bool)*bool*(bool array)>
+    ((0, !t1 ^^ fst (snd (fst query1))),
+      (2, rand), false, tweak 0 (!t1 ^^ fst (snd (fst query1))) tau1) __nil).
+    (* END UGLY *)
+
+    rewrite (_:Dkc.Dkc.b{1} = false);[trivial|].
+    simplify.
+    intros keynt1 keynt2; split;[trivial|];intros eqkeynt inkeynt.
+    intros key_nt_tau inkey_nt_tau.
+
+    (* UGLY *)
+
+rewrite (hd_def<:Dkc.key*Dkc.key*Dkc.cipher>
+(proj Map.empty.[(0,
+    t1 ^^ fst (snd (fst query1))) <- keyt1].[(0,
+    !t1 ^^ fst (snd (fst query1))) <- keynt1].[(0,
+    !t1 ^^ fst (snd (fst query1)))],
+
+    proj Map.empty.[(0,
+      t1 ^^ fst (snd (fst query1))) <- keyt1].[(0,
+      !t1 ^^ fst (snd (fst query1))) <- keynt1].[(2, rand)],
+
+      Dkc.encode
+        (tweak 0 (!t1 ^^ fst (snd (fst query1))) tau1)
+        (proj Map.empty
+          .[(0,t1 ^^ fst (snd (fst query1))) <- keyt1]
+          .[(0,!t1 ^^ fst (snd (fst query1))) <- keynt1]
+          .[(0,!t1 ^^ fst (snd (fst query1)))]) 
+        keyTau1
+        (proj Map.empty.[(1, eval (fst (fst query1)) (fst (snd (fst query1)),
+          !snd (snd (fst query1)))) <- key_t_tau]
+        .[(2, rand) <- key_nt_tau]
+        .[(2, rand)])
+)
+
+(
+
+(proj Dkc.Dkc.kpub{1}.[(0,
+      t1 ^^ fst (snd (fst query1))) <- keyt1].[(0,
+      t1 ^^ fst (snd (fst query1)))],
+
+      proj Dkc.Dkc.kpub{1}.[(0,
+        t1 ^^ fst (snd (fst query1))) <- keyt1].[(1,
+        eval (fst (fst query1)) (fst (snd (fst query1)),
+          !snd (snd (fst query1))))],
+
+        Dkc.encode (tweak 0 (!t1 ^^ fst (snd (fst query1))) tau1) (proj Map.empty.[(0,
+          t1 ^^ fst (snd (fst query1))) <- keyt1].[(0,
+          t1 ^^ fst (snd (fst query1)))]) keyTau1 (proj Map.empty.[(1,
+          eval (fst (fst query1)) (fst (snd (fst query1)),
+            !snd (snd (fst query1)))) <- key_t_tau].[(1,
+          eval (fst (fst query1)) (fst (snd (fst query1)),
+            !snd (snd (fst query1))))])) ::
+      __nil)).
+
+    (* END UGLY *)
+    
+    delta hd.
+
+cut test : (forall (l : int list), let t::q = l in t = hd l).
+
+    simplify.
+
+
+end proof what follow contains old stuff
   rcondf {1} 27. admit.
   rnd.
   wp.
   rcondt {1} 18. admit.
   wp.
   rcondt {1} 19. admit.
+  rcondf {1} 20. admit.
   rcondt {1} 20. admit.
-  rcondt {1} 21. admit.
-  rnd.
   rnd.
   rnd.
   wp.
